RPCF/RPCF_syntax_rep.v
@@ -1,0 +1,132 @@
+
+Require Export CatSem.PCF.PCF_RMonad.
+Require Export CatSem.RPCF.RPCF_rep.
+
+Set Implicit Arguments.
+Unset Strict Implicit.
+Unset Transparent Obligations.
+Unset Automatic Introduction.
+
+
+Program Instance PCFE_rep_struct : 
+       PCFPO_rep_struct PCFEM  PCF.arrow PCF.Bool PCF.Nat := {
+  app r s := PCFApp r s;
+  abs r s := PCFAbs r s;
+  rec t := PCFRec t ;
+  tttt := PCFconsts ttt ;
+  ffff := PCFconsts fff;
+  Succ := PCFconsts succ;
+  Pred := PCFconsts preds;
+  CondN := PCFconsts condN;
+  CondB := PCFconsts condB;
+  Zero := PCFconsts zero ;
+  nats m := PCFconsts (Nats m);
+  bottom t := PCFbottom t
+}.
+Next Obligation.
+Proof.
+  unfold Rsubst_star_map.
+  simpl.
+  apply clos_refl_trans_1n_contains.
+  apply relorig.
+  apply app_abs.
+Qed.
+(*
+Next Obligation.
+Proof.
+  apply cp_App1.
+  auto.
+Qed.
+Next Obligation.
+Proof.
+  apply cp_App2.
+  auto.
+Qed.
+Next Obligation.
+Proof.
+  apply cp_Lam.
+  auto.
+Qed.
+Next Obligation.
+Proof.
+  apply cp_Rec.
+  auto.
+Qed.
+*)
+Next Obligation.
+Proof.
+  apply clos_refl_trans_1n_contains.
+  apply relorig.
+  constructor.
+Qed.
+Next Obligation.
+Proof.
+  apply clos_refl_trans_1n_contains.
+  apply relorig.
+  constructor.
+Qed.
+Next Obligation.
+Proof.
+  apply clos_refl_trans_1n_contains.
+  apply relorig.
+  constructor.
+Qed.
+Next Obligation.
+Proof.
+  apply clos_refl_trans_1n_contains.
+  apply relorig.
+  constructor.
+Qed.
+Next Obligation.
+Proof.
+  apply clos_refl_trans_1n_contains.
+  apply relorig.
+  constructor.
+Qed.
+Next Obligation.
+Proof.
+  apply clos_refl_trans_1n_contains.
+  apply relorig.
+  constructor.
+Qed.
+Next Obligation.
+Proof.
+  apply clos_refl_trans_1n_contains.
+  apply relorig.
+  constructor.
+Qed.
+Next Obligation.
+Proof.
+  apply clos_refl_trans_1n_contains.
+  apply relorig.
+  constructor.
+Qed.
+Next Obligation.
+Proof.
+  apply clos_refl_trans_1n_contains.
+  apply relorig.
+  constructor.
+Qed.
+Next Obligation.
+Proof.
+  apply clos_refl_trans_1n_contains.
+  apply relorig.
+  constructor.
+Qed.
+
+
+Definition PCFE_rep : PCFPO_rep := 
+  Build_PCFPO_rep (type_type:=TY) (type_arrow:=PCF.arrow)
+   (pcf_rep_monad:=PCFEM)
+   PCFE_rep_struct.
+
+
+
+
+
+
+
+
+
+
+
